coq/SystemFTest.v
@@ -13,7 +13,13 @@ From ExtLib Require Import
      Structures.Functor
      Eqv.
 
+From Vellvm Require Import
+     Numeric.Integers
+     Utils.Util.
+
 Require Import SystemF.
+Require Import Lia.
+
 
 Import ListNotations.
 Import MonadNotation.
@@ -93,13 +99,14 @@ Fixpoint showTerm_helper {I} `{FInt I} `{Show I} (prec : Precedence) (e : Term) 
     parens prec oprec (showTerm_helper oprec e1 ++ " " ++ show op ++ " " ++ showTerm_helper oprec e2) 
   end.
 
+Instance showInt64 : Show Int64.int :=
+  {| show := fun i => show (Int64.intval i)
+  |}.
+
 Instance showTerm {I} `{FInt I} `{Show I} : Show Term :=
   {| show := showTerm_helper PrecOuter
   |}.
 
-Require Import Lia.
-
-Check map TVar (map N.of_nat (seq 0 1)).
 
 Definition elems_fail {A : Type} (l : list A) :=
   let n := length l in
@@ -127,3 +134,221 @@ Next Obligation.
 Admitted.
 Next Obligation.
 Admitted.
+
+Definition genFType (ftv : nat) : G FType
+  := sized (genFType' ftv).
+
+(* ** FType Tests ** *)
+Definition ftype_eq_refl (τ : FType) : bool
+  := ftype_eq τ τ.
+
+QuickCheck (forAll (genFType 10) ftype_eq_refl).
+
+Definition genInt64 : G Int64.int
+  := z <- arbitrary;;
+     ret (Int64.repr z).
+
+Definition genIfType {A} (τ1 τ2 : FType) (g : G A) : list (G A)
+  := if ftype_eq τ1 τ2 then [g] else [].
+
+Definition guard (b : bool) : list unit
+  := if b
+     then [tt]
+     else [].
+
+
+Compute guard (ftype_eq IntType (TVar 2));; ret 2.
+
+Fixpoint addIndices' {A} (i : N) (l : list A) : list (N * A)
+  := match l with
+     | nil => nil
+     | (x::xs) => (i,x) :: addIndices' (N.succ i) xs
+     end.
+
+Definition addIndices {A} := @addIndices' A 0.
+
+(* Probably want a variant of this that won't make recursive calls *)
+Program Fixpoint genTerm' (ftv : nat) (Γ : list FType) (τ : FType) (sz : N) : G Term
+  :=
+    match sz with
+    | N0 =>
+      oneOf_ failGen
+             ( (guard (ftype_eq IntType τ);; ret (fmap Num genInt64)) ++
+               (* Generate variables from the context with the same type *)
+               ('(i,τ') <- addIndices Γ;; guard (ftype_eq τ' τ);; ret (returnGen (Var i))) ++
+               (* Generate fixpoints... Need a way of ruling out recursive applications *)
+               (match τ with
+                | Arrow τ1 τ2 =>
+                  ret (arg <- genTerm' ftv (τ1 :: Γ) τ2 0;;
+                       returnGen (Fix τ1 arg))
+                | _ => []
+                end) ++
+               (match τ with
+                | TForall τ1 =>
+                  ret (
+                    )
+                | _ => []
+                end)
+               (* Tuples *)
+               
+             )
+    | Npos x => _
+    end.
+Next Obligation.
+Admitted.
+
+
+[ return $ Var i | (i,t') <- zip [0..] c, t == t' ] ++
+[ Lam t1 <$> arb ftv (t1:c) t2 0 | (t1 :-> t2) <- [t] ] ++
+[ TLam <$> arb (ftv+1) (map (liftType 0) c) t1 0 | (ForAll t1) <- [t] ]   -- MUTANT?
+
+  match sz with
+     | O =>
+     | S x => _
+     end.
+Inductive Term {I} `{FInt I} : Type :=
+| Var          : VarInd -> Term (* *)
+(* Annotated terms *)
+| Ann          : Term -> FType -> Term
+(* Terms *)
+| Fix          : FType -> Term -> Term (* *)
+| App          : Term -> Term -> Term
+(* Type stuff *)
+| TAbs         : Term -> Term
+| TApp         : Term -> FType -> Term
+(* Prod *)
+| Tuple        : list Term -> Term 
+| ProjN        : N -> Term -> Term
+(* Int *)
+| Num          : I -> Term
+(* Expressions *)
+| If0          : Term -> Term -> Term -> Term
+| Op           : PrimOp -> Term -> Term -> Term
+.
+
+
+(* Want to be able to generate basic loops... But don't want general recursion...
+
+   Make it so I can rule out the variable for the recursive call.
+
+   Make it so that I can call recursively if the argument, n, has IntType,
+   and if I force the recursive call to be applied to (n-1), *AND* the body
+   of the fix starts with if0.
+ *)
+(* Fix τ
+    (if0 (Var 1) (* this is the argument to fix *)
+    (call with Var 0 (f), and then (Var 1 - Num 1)) (* Make a decreasing call *)
+    (something-that-can't-access Var 0)
+     )
+*)
+
+Definition factorial : @Term Int64.int FInt64
+  := Fix IntType
+         (If0 (Var 1)
+              (Num (Int64.repr 1))
+              (Op Mul (App (Var 0) (Op Sub (Var 1) (Num (Int64.repr 1)))) (Var 1))).
+
+Definition step' (v : unit + Term) : (unit + Term)
+  := match v with
+     | inl tt => inl tt
+     | inr t => step t
+     end.
+
+Fixpoint multistep (n : nat) (v : Term) : Term
+  := match n with
+     | O => v
+     | S n =>
+       match step v with
+       | inl tt => v
+       | inr t => multistep n t
+       end
+     end.
+
+Compute (multistep 100 (App factorial (Num (Int64.repr 3)))).
+
+(*       
+genExpr :: _ => Gen Expr
+genExpr =
+--  traceShow (?config, ?mutant) $
+  (gcTake ?config) $ sized $ (\n -> do t <- genType 0; arb 0 [] t n)
+    where arb :: Int -> [Type] -> Type -> Int -> Gen Expr
+          arb ftv c t 0 = (gcBaseChoice ?config) $
+                          [ return Con | t == Base ] ++
+--                          [ return BTrue | t == TBool ] ++
+--                          [ return BFalse | t == TBool ] ++                          [ return $ Var i | (i,t') <- zip [0..] c, t == t' ] ++
+                          [ Lam t1 <$> arb ftv (t1:c) t2 0 | (t1 :-> t2) <- [t] ] ++
+                          [ TLam <$> arb (ftv+1) (map (liftType 0) c) t1 0 | (ForAll t1) <- [t] ]   -- MUTANT?
+          arb ftv c t n = (takeG $ gcRecChoiceTake ?config) . (gcRecChoice ?config) $
+                          [ (6, arb ftv c t 0) ] ++
+                          [ (8, Lam t1 <$> (arb ftv (t1:c) t2 (n-1))) | (t1 :-> t2) <- [t] ] ++
+                          [ (4, TLam <$> (arb (ftv+1) (map (liftType 0) c) t1 (n-1))) | (ForAll t1) <- [t] ] ++
+                          [ (8, do t2 <- retry (gcRetryType ?config) $ do
+                                         arbT <- resize 10 $ genType ftv   -- for now; should be bigger?
+                                         -- TODO: Michal?
+                                         elements (nub $ michal c t ++ [arbT])
+                                   nr <- choose (1,2)
+                                   me1 <- retry nr $ arb ftv c (t2 :-> t) (n `div` 2)
+                                   me2 <- arb ftv c t2 (n `div` 2)
+                                   return $ me1 :@: me2) ] ++
+                          [ (4, do (t1, t2) <- retry (gcRetryTApp ?config) $ genT1T2 t
+                                   me1 <- arb ftv c t1 (n - 1)
+                                   return $ TApp me1 t2) ] {- ++
+                         [ (1, do e1 <- arb ftv c TBool (n `div` 3)
+                                  e2 <- arb ftv c t (n `div` 3)
+                                  e3 <- arb ftv c t (n `div` 3)
+                                  return $ Cond e1 e2 e3) ] -}
+
+
+michal c t = [t' | varType <- c,
+                   t' <- aux varType]
+  where aux (t1 :-> t2) | t==t2 = [t1]
+                        | t/=t2 = aux t2
+        aux _                   = []
+
+
+-- Check if a type has any type variables.
+-- TODO: replace with "isClosed"
+hasTVars :: Type -> Bool
+hasTVars (TVar _)    = True
+hasTVars (t1 :-> t2) = hasTVars t1 || hasTVars t2
+hasTVars (ForAll t)  = hasTVars t
+hasTVars TBool       = False
+hasTVars Base        = False
+
+
+isClosed :: Type -> Bool
+isClosed = isClosed' 0
+  where
+    isClosed' :: Int -> Type -> Bool
+    isClosed' tc (TVar x)    = x < tc
+    isClosed' tc (t1 :-> t2) = isClosed' tc t1 && isClosed' tc t2
+    isClosed' tc (ForAll t)  = isClosed' (tc+1) t
+    isClosed' _ TBool        = True
+    isClosed' _ Base         = True
+
+-- Randomly fetch a subterm of a type
+fetchSubType :: Type -> Gen Type
+fetchSubType t =
+  oneof $
+  [ return t | isClosed t ] ++
+  [ fetchSubType t1 | (t1 :-> t2) <- [t] ] ++
+  [ fetchSubType t2 | (t1 :-> t2) <- [t] ] ++
+  [ fetchSubType t' | (ForAll t') <- [t] ]
+
+replaceSubType :: Int -> Type -> Type -> Gen Type
+-- "Replace (some occurrences of) closed type s in type t by (TVar n)"
+replaceSubType n s t =
+  oneof $
+  [ return t ] ++
+  [ return $ TVar n | s == t ] ++
+  [ do t1' <- replaceSubType n s t1; t2' <- replaceSubType n s t2; return $ t1' :-> t2' | (t1 :-> t2) <- [t] ] ++
+  [ do t'' <- replaceSubType (n+1) s t'; return $ ForAll t'' | (ForAll t') <- [t], t' == s ]
+
+-- Generate t1 t2 such that t1{0:=t2} = t
+genT1T2 :: Type -> Gen (Type, Type)
+genT1T2 t = do
+  let t' = let ?mutant = NoMutant in liftType 0 t
+  t2 <- fetchSubType t'
+  t1 <- replaceSubType 0 t2 t'
+  return (ForAll t1, t2)
+*) 
